examples/pseudo_bool/pb_parseScript.sml
@@ -19,8 +19,8 @@ Definition lhs_string_def:
 End
 
 Definition pbc_string_def:
-  (pbc_string (Equal xs i) = concat [lhs_string xs; strlit " = "; int_to_string #"-" i]) ∧
-  (pbc_string (GreaterEqual xs i) = concat [lhs_string xs; strlit " >= "; int_to_string #"-" i])
+  (pbc_string (Equal xs i) = concat [lhs_string xs; strlit " = "; int_to_string #"-" i; #";"]) ∧
+  (pbc_string (GreaterEqual xs i) = concat [lhs_string xs; strlit " >= "; int_to_string #"-" i; #";"])
 End
 
 (* TODO: move below into pb_parse *)
